---
tags: [OpenLearn/Week 3]
title: Brackets in mathematics
created: '2021-06-23T21:12:29.520Z'
modified: '2021-07-22T21:23:37.207Z'
---

# Brackets in mathematics

As you have seen, brackets are used to indicate, and clarify, the order in which a numerical calculation should be carried out. This is also true when you are using symbols, as in algebra.

So, for example considering $2(2n + 5)$ you should first multiple out the brackets. This means that all of the expression inside the brackets is multiplied by the figure outside them – a crucial idea to remember.

Thus:

$$2(2n + 5) = (2 \times 2n) + (2 \times 5) \\ \ \\
= 4n + 10$$

Here's another example:

$$a - 2(a - 3) =  \\ \ \\
= a - 2a + 6 \\ \ \\
= -a + 6$$

Things become more complicated when you need to multiply two expressions both within brackets. For this you have to multiply each term, in both brackets by each other.

Let’s consider this example:

$$(a + 2)(b - 1)$$

If you remember the acronym **FOIL**, this helps remember all the steps for multiplying the:
**F**irst elements
**O**utside elements
**I**nside elements
**L**ast elements

in the brackets. The expression above then becomes:

$$(a + 2)(b - 1) \\ \ \\
= ab - a + 2b - 2$$

## Exercises

Expand each of the following expressions by removing the brackets. Then (if possible) collect like terms.

1) $2(2x – y)$
> $4x - 2y$

2) $–2(a + 2b – c)$
> $-2a -4b + 2c$

3) $4(r + 6s) – (4s – r)$
> $4r + 24s - 4s + r = 5r + 20s$

4) $x(2x – 3) – 2x(5 – 2x)$
> $2x^2 - 3x - 10x + 4x^2 = 6x^2 - 13x$

5) $(x – 2)(x + 3)$
>  $x^2 + 3x - 2x -6 = x^2 + x -6$

6) $(r+t)^2$
> $(r + t)(r + t) = r^2 + rt + rt + t^2 = r^2 + t^2 + 2rt$

7) $(a – 4)(a + 4)$
> $a^2 + 4a -4a -16 = a^2 -16$

8) $\frac{1}{3}(p - 6)^2$
> $\frac{1}{3}( (p - 6)(p - 6) ) = \frac{1}{3}(p^2 - 6p - 6p + 36) = \frac{1}{3}p^2 - 4p + 12$





